adding alternative operational semantics

src/extensions/paths/OperationalSemantics.v
@@ -5,40 +5,40 @@ Require Import Definitions Binding Lookup.
 
 (** * Stack-Based Operational Semantics *)
 
-Reserved Notation "t1 '|->' t2" (at level 40, t2 at level 39).
+Reserved Notation "t1 '|=>' t2" (at level 40, t2 at level 39).
 
-Inductive red : sta * trm -> sta * trm -> Prop :=
+Inductive red' : sta * trm -> sta * trm -> Prop :=
 
 (** [s ∋ (p, lambda(T)t)  ]      #<br>#
     [―――――――――――――――――――――]      #<br>#
-    [(s, p q) |-> (s, t^q)]      *)
-| red_app: forall s p q T t,
-    s ∋ (p, val_lambda T t) ->
-    (s, trm_app p q) |-> (s, open_trm_p q t)
+    [(s, p q) |=> (s, t^q)]      *)
+| red'_app: forall s p q T t,
+    s ∋ (p, λ(T) t) ->
+    (s, trm_app p q) |=> (s, open_trm_p q t)
 
-(** [(s, let x = v in t) |-> ((s, x = v), t^x)] *)
-| red_let_val : forall v t s x,
+(** [(s, let x = v in t) |=> ((s, x = v), t^x)] *)
+| red'_let_val : forall v t s x,
     x # s ->
-    (s, trm_let (trm_val v) t) |-> (s & x ~ v, open_trm x t)
+    (s, trm_let (trm_val v) t) |=> (s & x ~ v, open_trm x t)
 
-(** [(s, let y = p in t) |-> (s, t^p)] *)
-| red_let_path : forall t s p,
-    (s, trm_let (trm_path p) t) |-> (s, open_trm_p p t)
+(** [(s, let y = p in t) |=> (s, t^p)] *)
+| red'_let_path : forall t s p,
+    (s, trm_let (trm_path p) t) |=> (s, open_trm_p p t)
 
-(** [(s, t0) |-> (s', t0')]                            #<br>#
+(** [(s, t0) |=> (s', t0')]                            #<br>#
     [―――――――――――――――――――――――――――――――――――――――――――――――]  #<br>#
-    [(s, let x = t0 in t) |-> (s', let x = t0' in t)]  *)
-| red_let_tgt : forall t0 t s t0' s',
-    (s, t0) |-> (s', t0') ->
-    (s, trm_let t0 t) |-> (s', trm_let t0' t)
+    [(s, let x = t0 in t) |=> (s', let x = t0' in t)]  *)
+| red'_let_tgt : forall t0 t s t0' s',
+    (s, t0) |=> (s', t0') ->
+    (s, trm_let t0 t) |=> (s', trm_let t0' t)
 
-where "t1 '|->' t2" := (red t1 t2).
+where "t1 '|=>' t2" := (red' t1 t2).
 
 (** ** Normal forms *)
 
-(** Paths and values are considered to be in normal form. *)
+(** Paths and values are considered' to be in normal form. *)
 Inductive norm_form: trm -> Prop :=
 | nf_path: forall p, norm_form (trm_path p)
 | nf_val: forall v, norm_form (trm_val v).
 
-Hint Constructors red norm_form.
+Hint Constructors red' norm_form.
