src/extensions/paths-no-closure-os/CanonicalForms.v
@@ -1,0 +1,834 @@
+(** printing |-#    %\vdash_{\#}%    #&vdash;<sub>&#35;</sub>#     *)
+(** printing |-##   %\vdash_{\#\#}%  #&vdash;<sub>&#35&#35</sub>#  *)
+(** printing |-##v  %\vdash_{\#\#v}% #&vdash;<sub>&#35&#35v</sub># *)
+(** printing |-!    %\vdash_!%       #&vdash;<sub>!</sub>#         *)
+(** remove printing ~ *)
+
+(** This module proves the Canonical Forms Lemmas, which allow us
+    to retrieve the shape of a value given its type. *)
+
+Set Implicit Arguments.
+
+Require Import Coq.Program.Equality List.
+Require Import Binding Definitions GeneralToTight InvertibleTyping Lookup Narrowing PreciseTyping
+        Replacement ReplacementTyping RecordAndInertTypes Substitution Subenvironments TightTyping
+        Weakening.
+Require Import Sequences.
+
+Definition deftrm t : trm :=
+  match t with
+  | defp p => trm_path p
+  | defv v => trm_val v
+  end.
+
+(** * Lemmas to prove that [γ ⟦ p ↦ t ⟧] and [Γ ⊢! p: T] imply [Γ ⊢ t: T] *)
+
+Lemma repl_composition_sub G T U :
+  G ⊢ T ⟿ U ->
+  G ⊢ U <: T /\ G ⊢ T <: U.
+Proof.
+  intros Hr. dependent induction Hr; eauto.
+  destruct H as [q [r [n [S [Hq%precise_to_general [Hq' Hrt]]]]]]. destruct_all.
+  split.
+  - eapply subtyp_trans. apply* subtyp_sngl_qp. apply* precise_to_general2. eauto.
+  - eapply subtyp_trans. apply H0. apply repl_swap in Hrt. eapply subtyp_sngl_pq; eauto. apply* precise_to_general2.
+Qed.
+
+Lemma defs_invert_trm x bs G d a T :
+  x; bs; G ⊢ d : {a ⦂ T} ->
+  exists t, d = {a := t}.
+Proof.
+  intros Hd. inversion Hd; eauto.
+Qed.
+
+Lemma object_typing G x bs ds T a t V :
+  inert G ->
+  x; bs; G ⊢ ds :: T ->
+  defs_has ds {a := t} ->
+  record_has T {a ⦂ V} ->
+  (exists U u, t = defv (λ(U) u) /\ G ⊢ deftrm t : V) \/
+  (exists U ds', t = defv (ν(U) ds') /\
+            x; (a :: bs); G ⊢ open_defs_p (p_sel (avar_f x) (a :: bs)) ds' ::
+                                 open_typ_p (p_sel (avar_f x) (a :: bs)) U /\
+            V = μ U) \/
+  (exists q S, t = defp q /\ V = {{ q }} /\ G ⊢ trm_path q : S).
+Proof.
+  intros Hi Hds Hdh Hr.
+  destruct (record_has_ty_defs Hds Hr) as [? [Hdh' Hdt]].
+  destruct (defs_invert_trm Hdt) as [t' ->].
+  pose proof (defs_has_inv Hdh Hdh') as <-. destruct t as [q | v]; simpl in *.
+  - inversion* Hdt.
+  - destruct v.
+    * right. left. inversions Hdt.
+      simpl in *. repeat eexists; auto.
+    * left. inversions Hdt. eauto.
+Qed.
+
+Lemma pt3_exists G p T :
+  inert G ->
+  G ⊢ trm_path p : T ->
+  exists U, G ⊢!!! p : U.
+Proof.
+  intros Hi Hp. apply (general_to_tight_typing Hi) in Hp.
+  apply tight_to_prec_exists in Hp as [? ?]; eauto.
+Qed.
+
+Lemma lookup_step_preservation_prec1: forall G s p px pbs t T U,
+    inert G ->
+    wf_env G ->
+    well_typed G s ->
+    s ⟦ p ⟼ t ⟧ ->
+    G ⊢! p : T ⪼ U ->
+    p = p_sel (avar_f px) pbs ->
+    (exists S u, t = defv (λ(S) u) /\ G ⊢ deftrm t : T) \/
+    (exists S ds W T' G1 G2 pT,
+        t = defv (ν(S) ds) /\
+        T = μ T' /\
+        G = G1 & px ~ pT & G2 /\
+        px ; pbs; G ⊢ open_defs_p p ds :: open_typ_p p S /\
+        G1 ⊩ S ⟿ W ⬳ T') \/
+    (exists q r r' G1 G2 pT,
+        t = defp q /\
+        T = {{ r }} /\
+        G = G1 & px ~ pT & G2 /\
+        (r = r' \/ G1 ⊢!!! r : {{ r' }}) /\ (q = r' \/ G1 ⊢!!! q : {{ r' }})).
+Proof.
+  introv Hi Hwf Hwt. gen p px pbs t T U.
+  (** induction on well-formedness **)
+  induction Hwt; introv Hs Hp Heq.
+  - Case "G is empty".
+    false* lookup_empty.
+  - Case "G is not empty".
+    pose proof (typed_paths_named (precise_to_general Hp)) as [px' [bs ->]].
+    destruct (classicT (x = px')) as [-> | Hn].
+    * SCase "x = px".
+      (** induction on ⟦⟼⟧ **)
+      gen T U T0 px pbs.
+      dependent induction Hs; introv Hwf Hi Hv; introv Hp; introv [= -> <-];
+        try simpl_dot; try rewrite proj_rewrite in *.
+      + SSCase "lookup_var".
+        apply binds_push_eq_inv in H1 as ->.
+        lets Hb: (pf_binds Hi Hp). pose proof (binds_push_eq_inv Hb) as ->.
+        apply binds_inert in Hb; auto.
+        destruct v as [S ds | S u].
+        ++ right. left.
+           lets Hi': (inert_prefix Hi). lets Hwf': (wf_env_prefix Hwf).
+           inversions Hb; proof_recipe. { inversion Hvpr. }
+           inversions Hv. pick_fresh z. assert (z \notin L) as Hz by auto.
+           apply H4 in Hz. repeat eexists.
+           +++ rewrite concat_empty_r. eauto.
+           +++ apply open_env_last_defs; auto.
+               apply narrow_defs with (G:=G & px ~ open_typ px S). {
+                 assert (open_defs_p (p_sel (avar_f px) nil) ds = open_defs px ds) as -> by rewrite* open_var_defs_eq.
+                 assert (open_typ_p (p_sel (avar_f px) nil) S = open_typ px S) as -> by rewrite* open_var_typ_eq.
+                 apply rename_defs with (x := z); auto.
+               }
+               apply subenv_last; auto. apply (repl_composition_open (pvar px)) in Hrc.
+               eapply (repl_composition_open (pvar px)) in Hrc'.
+               apply subtyp_trans with (T:=open_typ px U');
+                 apply repl_composition_sub in Hrc'; apply repl_composition_sub in Hrc; destruct_all;
+                   repeat rewrite open_var_typ_eq in *; unfold pvar in *; auto. all: auto.
+           +++ eauto.
+           +++ eauto.
+        ++ left. repeat eexists. apply* weaken_ty_trm.
+      + SSCase "lookup_sel_p".
+        destruct (pf_invert_fld _ _ Hp) as [V Hp'].
+        specialize (IHHs _ _ _ Hwt IHHwt _ H0 H JMeq_refl eq_refl _ Hwf Hi Hv _ _ Hp' _ _ eq_refl)
+          as [[? [? [[=] ?]]] |
+              [[? [? [? [? [? [? [? [[=]]]]]]]]] |
+               [? [? [? [? [? [? [[= ->] [-> [[= ->] ?]]]]]]]]]]].
+        apply pf_sngl_U in Hp'. inversion Hp'.
+      + SSCase "lookup_sel_v".
+        destruct (pf_invert_fld _ _ Hp) as [V Hp'].
+        specialize (IHHs _ _ _ Hwt IHHwt _ H0 H JMeq_refl eq_refl _ Hwf Hi Hv _ _ Hp' _ _ eq_refl)
+          as [[? [? [[=] ?]]] |
+              [[S [ds' [W [T'' [G1 [G2 [pT [[= -> ->] [[= ->] [Heq [Hds Hrc]]]]]]]]]]] |
+               [? [? [? [? [? [? [[= ->] [-> [[= ->] ?]]]]]]]]]]].
+        lets H': (defs_has_open (p_sel (avar_f px) f) H1). simpl in *.
+        lets Hr: (pf_record_has_U Hi Hp').
+        rewrite Heq in Hi, Hwf.
+        pose proof (repl_comp_trans_open (p_sel (avar_f px) f)
+                                         (inert_prefix (inert_prefix Hi))
+                                         Hrc) as Hrc_op.
+        pose proof (repl_comp_trans_record_has Hrc_op Hr) as [V [W' [Hrh [Hrc1' Hrc2']]]].
+        rewrite <- concat_empty_r in Heq at 1.
+        assert (G2 = empty) as ->. {
+          eapply env_ok_inv. eauto. rewrite concat_empty_r. rewrite <- Heq, concat_empty_r in Hi. auto.
+        }
+        repeat rewrite concat_empty_r in *. apply eq_push_inv in Heq as [_ [<- <-]].
+        assert (G & px ~ T0 ⊢ V <: T1 /\ G & px ~ T0 ⊢ T1 <: V) as [HVT HTV]. {
+          apply repl_composition_sub in Hrc2'. apply repl_composition_sub in Hrc1'.
+          destruct_all.
+          split; apply weaken_subtyp; eauto.
+        }
+        destruct (object_typing Hi Hds H' Hrh) as [[U' [u [Heq Ht']]] |
+                                                   [[U' [ds'' [Heq [Hds'' ->]]]] | [q [V' [Heq1 [-> Hq]]]]]].
+        ++ destruct t; inversions Heq. destruct v0; inversions H3.
+           left. repeat eexists. eauto.
+        ++ destruct t as [|]; inversions Heq. destruct v0 as [X ds |]; inversions H3. fold open_rec_defs_p in Hds''.
+           right. left.
+           pose proof (repl_comp_bnd_inv1 Hrc1') as [Y ->]. pose proof (repl_comp_bnd_inv2 Hrc2') as [Z ->].
+           repeat eexists; eauto.
+           +++ apply repl_comp_bnd' in Hrc1'. rewrite concat_empty_r. eauto.
+           +++ apply repl_comp_bnd' in Hrc1'. apply Hrc1'.
+           +++ apply* repl_comp_bnd'.
+        ++ destruct t; inversions Heq1. right. right.
+           pose proof (repl_comp_sngl_inv1 Hrc1') as [r ->]. pose proof (repl_comp_sngl_inv2 Hrc2') as [r' ->].
+           pose proof (pf_sngl_U Hp) as ->.
+           pose proof (sngl_typed Hi Hwf Hp) as [V Hr'%pt3].
+           pose proof (pt3_exists Hi Hq) as [V'' Hp3].
+           pose proof (repl_comp_to_prec' Hi Hwf Hrc2' Hr')
+             as [-> | Hpr];
+             pose proof (repl_comp_to_prec' Hi Hwf Hrc1' Hp3)
+             as [<- | Hpr']; clear Hrc1' Hrc2';
+               repeat eexists; try rewrite concat_empty_r; eauto.
+    * SCase "x <> x0".
+      apply pf_strengthen in Hp; auto. apply lookup_strengthen_one in Hs; auto.
+      inversions Heq.
+      specialize (IHHwt (inert_prefix Hi) (wf_env_prefix Hwf) _ _ _ _ _ _ Hs Hp eq_refl)
+        as [[? [? [[= ->]]]] |
+              [[? [? [? [? [? [? [? [-> [-> [-> [Hds [? ?]]]]]]]]]]]] |
+               [? [? [? [? [? [? [[= ->] [[= ->] [-> [? ?]]]]]]]]]]]].
+      + left. repeat eexists. apply* weaken_ty_trm.
+      + right. left. repeat eexists. rewrite concat_assoc. eauto.
+        apply* weaken_ty_defs. all: eauto.
+      + right. right. repeat eexists. rewrite concat_assoc. all: eauto.
+Qed.
+Lemma lookup_step_preservation_prec2 G s p px pbs t T :
+    inert G ->
+    wf_env G ->
+    well_typed G s ->
+    s ⟦ p ⟼ t ⟧ ->
+    G ⊢!! p : T ->
+    p = p_sel (avar_f px) pbs ->
+    (exists S U u, t = defv (λ(S) u) /\ G ⊢ deftrm t : U /\ G ⊢! p : U ⪼ T) \/
+    (exists S ds W U G1 G2 pT,
+        t = defv (ν(S) ds) /\
+        G ⊢! p : μ U ⪼ T /\
+        G = G1 & px ~ pT & G2 /\
+        px ; pbs; G ⊢ open_defs_p p ds :: open_typ_p p S /\
+        G1 ⊩ S ⟿ W ⬳ U) \/
+    (exists q r r' G1 G2 pT,
+        t = defp q /\
+        T = {{ r }} /\
+        G = G1 & px ~ pT & G2 /\
+        (r = r' \/ G1 ⊢!!! r : {{ r' }}) /\ (r' = q \/ G1 ⊢!!! q : {{ r' }})).
+Proof.
+  introv Hi Hwf Hwt Hs Hp Heq. gen s t px pbs. induction Hp; introv Hwt; introv Hs; introv Heq.
+  - destruct (lookup_step_preservation_prec1 Hi Hwf Hwt Hs H Heq)
+      as [[? [? [[= ->]]]] |
+          [[S [ds' [W [T'' [G1 [G2 [pT [-> [-> [-> [Hds [Hrc1 Hrc2]]]]]]]]]]]] |
+           [? [? [? [? [? [? [-> [-> [-> [? ?]]]]]]]]]]]].
+    * left. repeat eexists; eauto.
+    * right. left. repeat eexists; eauto.
+    * pose proof (pf_sngl_U H) as ->. right. right. repeat eexists; eauto.
+      destruct_all; eauto.
+  - clear IHHp2. simpl_dot. specialize (IHHp1 Hi Hwf _ Hwt).
+    gen q U. dependent induction Hs; simpl_dot; introv Hp IHHp1 Hv.
+    * specialize (IHHp1 _ Hs _ _ eq_refl) as [[? [? [? [[=] ?]]]] |
+                                  [[? [? [? [? [? [? [? [[=] ?]]]]]]]] |
+                                   [q' [r [r' [G1 [G2 [pT [[= <-] [[= ->] [-> [Hrc1 Hrc2]]]]]]]]]]]].
+      right. right. exists (q • a) (r • a).
+      pose proof (inert_prefix (inert_prefix Hi)) as Hi'.
+      pose proof (wf_env_prefix (wf_env_prefix Hwf)) as Hwf'.
+      destruct Hrc1 as [-> | Hr1]; destruct Hrc2 as [-> | Hr2].
+      ** repeat eexists; eauto.
+      ** repeat eexists; eauto. right. apply* pt3_field_elim_p.
+         apply* pt3_trans2.
+         pose proof (sngl_typed3 Hi' Hwf' Hr2) as [_ [T Ht]%pt2_exists].
+         constructor. rewrite <- concat_assoc in *. apply* pt2_fld_strengthen.
+      ** repeat eexists. right. apply* pt3_field_elim_p.
+         rewrite <- concat_assoc in *. apply* pt3_fld_strengthen.
+         left*.
+      ** pose proof (field_elim_q3) as Hf.
+         rewrite <- concat_assoc in *.
+         pose proof (pt3_weaken (inert_ok Hi) Hr1).
+         specialize (Hf _ _ _ _ _ Hi H (pt3 Hv)) as [S Ht].
+         repeat eexists. rewrite* concat_assoc.
+         right. apply* pt3_field_elim_p.
+         apply* pt3_fld_strengthen.
+         right. apply* pt3_field_elim_p. apply* pt3_fld_strengthen.
+         eapply pt3_trans2. eapply pt3_weaken. apply* inert_ok. apply Hr2.
+         eapply pt3_weaken in Hr1. apply Ht. apply* inert_ok.
+    * specialize (IHHp1 _ Hs) as [[? [? [? [[= ->] ?]]]] |
+                                  [[? [? [? [? [? [? [? [? [[=]%pf_sngl_T [[=] [HH [HHH ?]]]]]]]]]]]] |
+                                   [? [? [? [? [? [? [[=] ?]]]]]]]]]; auto.
+Qed.
+Lemma lookup_step_preservation_inert_prec3: forall G s p T t,
+    inert G ->
+    wf_env G ->
+    well_typed G s ->
+    s ⟦ p ⟼ t ⟧ ->
+    G ⊢!!! p : T ->
+    inert_typ T ->
+    (exists S U, T = ∀(S) U /\ G ⊢ deftrm t : ∀(S) U) \/
+    (exists U, T = μ U /\
+          ((exists S ds px pbs W, t = defv (ν(S) ds) /\
+                               p = p_sel (avar_f px) pbs /\
+                               px; pbs; G ⊢ open_defs_p p ds :: open_typ_p p S /\
+                               G ⊩ S ⟿ W ⬳ U) \/
+           (exists q, t = defp q /\ G ⊢!!! q : T))).
+Proof.
+  introv Hi Hwf Hwt Hs Hp. gen t.
+  pose proof (typed_paths_named (precise_to_general3 Hp)) as [px [pbs Heq]].
+  dependent induction Hp; introv Hs Hit;
+    destruct (lookup_step_preservation_prec2 Hi Hwf Hwt Hs H Heq)
+                                as [[S' [U [u [[= ->] [Hv Hp']]]]] |
+                                    [[S' [ds [W [U [G1 [G2 [pT [[= ->] [Hp' [-> [Hds [Hrc1 Hrc2]]]]]]]]]]]] |
+                                     [q' [r [r' [G1 [G2 [pT [[= ->] [[= ->] [Heq' [Hrc1 Hrc2]]]]]]]]]]]]; simpl.
+  - left. simpl in *. inversions Hit.
+    * apply (pf_forall_T Hi) in Hp' as ->. repeat eexists; eauto.
+    * apply (pf_bnd_T Hi) in Hp' as ->. proof_recipe. inversion Hv.
+  - right. inversions Hit.
+    * apply (pf_forall_T Hi) in Hp' as [=].
+    * apply (pf_bnd_T Hi) in Hp' as [= ->]. eexists. split*. left. repeat eexists; eauto;
+      repeat apply* repl_composition_weaken; apply* inert_ok; apply* inert_prefix.
+  - inversion Hit.
+  - apply pf_sngl_T in Hp' as ->; auto. proof_recipe. false* repl_to_invertible_val_sngl.
+  - apply (pf_sngl_T Hi) in Hp' as [=].
+  - clear IHHp.
+    assert (exists V, G ⊢!!! q' : V) as [V Hq']. {
+      destruct Hrc1 as [-> | Hr]; destruct Hrc2 as [-> | Hr']; subst; rewrite <- concat_assoc in *; eauto.
+      - eexists. apply* pt3_weaken.
+      - apply sngl_typed3 in Hr as [S Ht]. eexists. apply* pt3_weaken. apply* inert_prefix. apply* wf_env_prefix.
+      - eexists. apply* pt3_weaken.
+    }
+    lets Hok: (inert_ok Hi). rewrite Heq' in Hok.
+    destruct Hrc1 as [-> | Hr]; destruct Hrc2 as [-> | Hr']; inversions Hit.
+    + left; repeat eexists; apply* precise_to_general3.
+    + right. eexists. split*.
+    + left. repeat eexists. apply* precise_to_general3. apply* pt3_sngl_trans3.
+      repeat apply* pt3_weaken.
+    + right. eexists. split*. right. eexists. split*.
+      apply* pt3_sngl_trans3. repeat apply* pt3_weaken.
+    + left. repeat eexists.
+      do 2 eapply pt3_weaken in Hr.
+      pose proof (pt3_inert_sngl_invert Hi Hp Hr (inert_typ_all _ _)) as Hr'.
+      apply* precise_to_general3. all: eauto; apply* inert_ok. apply* inert_prefix.
+    + right. eexists. split*. right. eexists. split*.
+      do 2 eapply pt3_weaken in Hr.
+      apply* (pt3_inert_sngl_invert Hi Hp Hr).
+      all: eauto; apply* inert_ok. apply* inert_prefix.
+    + left. repeat eexists. apply precise_to_general3.
+      eapply pt3_sngl_trans3. repeat apply* pt3_weaken.
+      apply* pt3_inert_sngl_invert. repeat apply* pt3_weaken.
+    + right. eexists. split*. right. eexists. split*.
+      eapply pt3_sngl_trans3. repeat apply* pt3_weaken.
+      apply* pt3_inert_sngl_invert. repeat apply* pt3_weaken.
+Qed.
+Lemma lookup_step_preservation_prec3_fun G s p T S t :
+  inert G ->
+  wf_env G ->
+  well_typed G s ->
+  s ⟦ p ⟼ t ⟧ ->
+  G ⊢!!! p : ∀(T) S ->
+  G ⊢ deftrm t : ∀(T) S.
+Proof.
+  intros Hi Hwf Hwt Hs Hp.
+  destruct (lookup_step_preservation_inert_prec3 Hi Hwf Hwt Hs Hp) as
+      [[? [? [-> Ht]]] | [? [[=] ?]]]; auto.
+Qed.
+
+(** * Lemmas to prove that [Γ ~ γ] and [Γ ⊢! p: T] imply [γ ∋ (p, v)] *)
+Lemma typ_to_lookup1 G s p T U :
+  inert G ->
+  wf_env G ->
+  well_typed G s ->
+  G ⊢! p : T ⪼ U ->
+  exists t, s ⟦ p ⟼ t ⟧.
+Proof.
+  intros Hi Hwf Hwt Hp. gen p T U. induction Hwt; introv Hp.
+  (** induction on ⟦~⟧ **)
+  - false. dependent induction Hp; eauto. apply* binds_empty_inv.
+  - pose proof (typed_paths_named (precise_to_general Hp)) as [y [bs ->]].
+    (* later when we figure out how to make env closed *)
+    destruct (classicT (x = y)) as [-> | Hn].
+    * SCase "x = y".
+      (** induction on ⟦⊢!⟧ **)
+      dependent induction Hp; try simpl_dot.
+      + eexists. apply* lookup_var.
+      + specialize (IHHp _ _ H0 _ _ Hwf Hi Hwt H H1 IHHwt JMeq_refl eq_refl) as [t Hs].
+        pose proof (pf_bnd_T2 Hi Hp) as [V ->].
+        destruct (lookup_step_preservation_prec1 Hi Hwf (well_typed_push Hwt H H0 H1) Hs Hp eq_refl)
+          as [[S [u [-> Ht]]] |
+              [[S [ds' [W [T'' [G1 [G2 [pT [-> [[= ->] ?]]]]]]]]] |
+               [? [? [? [? [? [? [? [[=] [? ?]]]]]]]]]]].
+        ++ proof_recipe. inversion Ht.
+        ++ assert (exists u, defs_has ds' {a := u}) as [u Hu]. {
+             destruct H3 as [Heq [Hds Hrc]].
+             apply pf_record_has_U in Hp; auto.
+             eapply repl_comp_trans_open in Hrc.
+             eapply repl_comp_trans_record_has in Hrc as [V [X [Hr _]]]; try apply Hp.
+             eapply record_has_ty_defs in Hds as [d [Hdh Hds]]; eauto.
+             eapply defs_invert_trm in Hds as [t ->]. unfold defs_has in *.
+             simpl in *. apply* defs_has_open'. rewrite  Heq in Hi, Hwf.
+             repeat apply* inert_prefix.
+           }
+           eexists. rewrite proj_rewrite. eauto.
+      + eauto.
+      + eauto.
+      + eauto.
+    * SCase "x <> y".
+      apply pf_strengthen in Hp; auto. specialize (IHHwt (inert_prefix Hi) (wf_env_prefix Hwf) _ _ _ Hp) as [t Hs].
+      eexists. apply* lookup_step_weaken_one.
+Qed.
+Lemma typ_to_lookup2 G s p T :
+  inert G ->
+  wf_env G ->
+  well_typed G s ->
+  G ⊢!! p : T ->
+  exists t, s ⟦ p ⟼ t ⟧.
+Proof.
+  intros Hi Hwf Hwt Hp. induction Hp.
+  - apply* typ_to_lookup1.
+  - specialize (IHHp1 Hi Hwf Hwt) as [u1 Hs1]. specialize (IHHp2 Hi Hwf Hwt) as [u2 Hs2].
+    pose proof (typed_paths_named (precise_to_general2 Hp1)) as [px [pbs ->]].
+    destruct (lookup_step_preservation_prec2 Hi Hwf Hwt Hs1 Hp1 eq_refl)
+                                as [[S' [U' [u [[= ->] [Hv Hp']]]]] |
+                                    [[S' [ds [W [U' [G1 [G2 [pT [-> [Hp' [Heq [Hds [Hrc1 Hrc2]]]]]]]]]]]] |
+                                     [? [? [? [? [? [? [-> [[= ->] ?]]]]]]]]]].
+    + pose proof (pf_sngl_T Hi Hp') as ->. proof_recipe. inversions Hv. inversions H. inversions H0.
+    + pose proof (pf_sngl_T Hi Hp') as [=].
+    + eauto.
+Qed.
+Lemma typ_to_lookup3 G s p T :
+  inert G ->
+  wf_env G ->
+  well_typed G s ->
+  G ⊢!!!p : T ->
+  exists t, s ⟦ p ⟼ t ⟧.
+Proof.
+  intros Hi Hwf Hwt Hp. induction Hp; apply* typ_to_lookup2.
+Qed.
+Lemma sngl_path_lookup1 G s p q U :
+  inert G ->
+  wf_env G ->
+  well_typed G s ->
+  G ⊢! p : {{ q }} ⪼ U ->
+           exists r r', s ⟦ p ⟼ defp r ⟧ /\
+                   (r = r' \/ G ⊢!!! r : {{ r' }}) /\
+                   (q = r' \/ G ⊢!!! q : {{ r' }}).
+Proof.
+  intros Hi Hwf Hwt Hp. destruct (typ_to_lookup1 Hi Hwf Hwt Hp) as [t Hs].
+  pose proof (typed_paths_named (precise_to_general Hp)) as [px [pbs ->]].
+  destruct (lookup_step_preservation_prec1 Hi Hwf Hwt Hs Hp eq_refl)
+           as [[S [u [-> Ht]]] |
+              [[S [ds' [W [T'' [G1 [G2 [pT [-> [[= ->] ?]]]]]]]]] |
+               [? [? [? [G1 [G2 [pT [-> [[= -> ] [-> [Hrc1 Hrc2]]]]]]]]]]]].
+  - proof_recipe. inversions Ht. inversions H. inversion H0.
+  - pose proof (inert_ok Hi) as Hok%ok_concat_inv_l.
+    destruct Hrc1 as [-> | Hx0]; destruct Hrc2 as [-> | Hrx1]; do 2 eexists; eauto.
+    + split*. split. right.
+      repeat apply* pt3_weaken. eauto.
+    + split*. split. left*. right. repeat apply* pt3_weaken.
+    + split*. split; right; repeat apply* pt3_weaken.
+Qed.
+Lemma lookup_step_preservation_sngl_prec3: forall G s p q t Q1 Q2 Q3,
+    inert G ->
+    wf_env G ->
+    well_typed G s ->
+    s ⟦ p ⟼ t ⟧ ->
+    G ⊢!!! p : {{ q }} ->
+    G ⊢! q : ∀(Q1) Q2 ⪼ Q3 ->
+    exists r r', t = defp r /\
+            (q = r' \/ G ⊢!!! q : {{ r' }}) /\
+            (r = r' \/ G ⊢!!! r : {{ r' }}).
+Proof.
+  introv Hi Hwf Hwt Hs Hp. gen t.
+  pose proof (typed_paths_named (precise_to_general3 Hp)) as [px [pbs Heq]].
+  dependent induction Hp; introv Hs Hq;
+    destruct (lookup_step_preservation_prec2 Hi Hwf Hwt Hs H Heq)
+    as [[S' [U' [u [[= ->] [Hv Hp']]]]] |
+        [[S' [ds [W [U [G1 [G2 [pT [-> [Hp' [Heq' [Hds [Hrc1 Hrc2]]]]]]]]]]]] |
+         [q' [r [r' [G1 [G2 [pT [-> [[= ->] [-> [Hrc1 Hrc2]]]]]]]]]]]].
+  - pose proof (pf_sngl_T Hi Hp') as ->. pose proof (sngl_path_lookup1 Hi Hwf Hwt Hp') as [? [? [Hl ?]]].
+    pose proof (lookup_step_func Hl Hs) as [=].
+  - pose proof (pf_sngl_T Hi Hp') as [=].
+  - destruct Hrc1 as [-> | Hrc1]; destruct Hrc2 as [-> | Hrc2]; do 2 eexists; eauto; split*; split;
+      [ left* | right | right | left* | right | right ]; repeat apply* pt3_weaken.
+    all: apply* inert_ok; apply* inert_prefix.
+  - pose proof (pf_sngl_T Hi Hp') as ->. pose proof (sngl_path_lookup1 Hi Hwf Hwt Hp') as [? [? [Hl ?]]].
+    pose proof (lookup_step_func Hl Hs) as [=].
+  - pose proof (pf_sngl_T Hi Hp') as [=].
+  - pose proof (typ_to_lookup3 Hi Hwf Hwt Hp) as [t Hl].
+    pose proof (typed_paths_named (precise_to_general3 Hp)) as [rx [rbs Heqr]].
+    specialize (IHHp _ Hi Hwf Hwt eq_refl _ _ Heqr _ Hl Hq) as [r1 [r2 [-> [[-> | Hq'] [-> | Hq'']]]]].
+      * destruct Hrc1 as [-> | Hp']; destruct Hrc2 as [-> | Hp'']; do 2 eexists; split*.
+        ** split. left*. right. apply* pt3_sngl_trans3. repeat apply* pt3_weaken.
+           apply inert_ok. apply* inert_prefix.
+        ** split. left*. do 2 eapply pt3_weaken in Hp'. pose proof (pt3_invert Hi Hp Hp')
+             as [? | [r1 [[= ->] [-> | ?]]]]; eauto.
+           false* pf_inert_pt3_sngl_false. all: apply* inert_ok; apply* inert_prefix.
+        ** split. left*. do 2 eapply pt3_weaken in Hp'; try solve [apply* inert_ok; apply* inert_prefix].
+           pose proof (pt3_invert Hi Hp Hp')
+             as [? | [r1 [[= ->] [-> | ?]]]].
+           *** right. apply* pt3_sngl_trans3. repeat apply* pt3_weaken. eapply inert_ok, inert_prefix; eauto.
+           *** right. repeat apply* pt3_weaken. eapply inert_ok, inert_prefix; eauto.
+           *** false* pf_inert_pt3_sngl_false.
+      * destruct Hrc1 as [-> | Hp']; destruct Hrc2 as [-> | Hp'']; do 2 eexists; split*.
+        ** split. left*. right. eapply pt3_sngl_trans3. repeat apply* pt3_weaken.
+           apply* inert_ok. apply* inert_prefix. auto.
+        ** split. left*. do 2 eapply pt3_weaken in Hp'; try solve [apply* inert_ok; apply* inert_prefix].
+           pose proof (pt3_invert Hi Hp Hp')
+             as [? | [r1' [[= ->] [-> | ?]]]]; eauto. false* pf_inert_pt3_sngl_false.
+        ** split. left*.
+           do 2 eapply pt3_weaken in Hp'; try solve [apply* inert_ok; apply* inert_prefix].
+           pose proof (pt3_invert Hi Hp Hp') as [? | [r1' [[= ->] [-> | HHH]]]].
+           *** right. apply* pt3_sngl_trans3. repeat apply* pt3_weaken. apply* inert_ok. apply* inert_prefix.
+           *** right. repeat apply* pt3_weaken. apply* inert_ok. apply* inert_prefix.
+           *** false* pf_inert_pt3_sngl_false.
+      * destruct Hrc1 as [-> | Hp']; destruct Hrc2 as [-> | Hp'']; do 2 eexists; split*.
+        ** split. left*. right. apply* pt3_sngl_trans3. repeat apply* pt3_weaken.
+           apply* inert_ok. apply* inert_prefix.
+        ** split. left*.
+           do 2 eapply pt3_weaken in Hp'; try solve [apply* inert_ok; apply* inert_prefix].
+           pose proof (pt3_invert Hi Hp Hp')
+             as [? | [r1 [[= ->] [-> | ?]]]]; eauto.
+           false* pf_inert_pt3_sngl_false.
+        ** split. left*.
+            do 2 eapply pt3_weaken in Hp'; try solve [apply* inert_ok; apply* inert_prefix].
+           pose proof (pt3_invert Hi Hp Hp')
+             as [? | [r1 [[= ->] [-> | ?]]]].
+           *** right. apply* pt3_sngl_trans3. repeat apply* pt3_weaken. apply* inert_ok; apply* inert_prefix.
+           *** right. repeat apply* pt3_weaken. apply* inert_ok; apply* inert_prefix.
+           *** false* pf_inert_pt3_sngl_false.
+      * destruct Hrc1 as [-> | Hp']; destruct Hrc2 as [-> | Hp'']; do 2 eexists; split*.
+        ** split. left*. right. eapply pt3_sngl_trans3. repeat apply* pt3_weaken.
+           apply inert_ok; apply* inert_prefix. auto.
+        ** split. left*.
+            do 2 eapply pt3_weaken in Hp'; try solve [apply* inert_ok; apply* inert_prefix].
+           pose proof (pt3_invert Hi Hp Hp')
+             as [? | [r1' [[= ->] [-> | ?]]]]; eauto. false* pf_inert_pt3_sngl_false.
+        ** split. left*.
+           do 2 eapply pt3_weaken in Hp'; try solve [apply* inert_ok; apply* inert_prefix].
+           pose proof (pt3_invert Hi Hp Hp') as [? | [r1' [[= ->] [-> | HHH]]]].
+           *** right. apply* pt3_sngl_trans3. repeat apply* pt3_weaken. apply* inert_ok. apply* inert_prefix.
+           *** right. repeat apply* pt3_weaken. apply* inert_ok. apply* inert_prefix.
+           *** false* pf_inert_pt3_sngl_false.
+Qed.
+
+Lemma lookup_same_var_same_type G s x bs cs T:
+  inert G ->
+  wf_env G ->
+  well_typed G s ->
+  s ⟦ p_sel (avar_f x) bs ⟼ defp (p_sel (avar_f x) cs) ⟧ ->
+  G ⊢!! p_sel (avar_f x) bs : T ->
+  T = {{ p_sel (avar_f x) cs }}.
+Proof.
+  intros Hi Hwf Hwt. gen x bs cs T. induction Hwt; introv Hs Ht.
+  - Case "s is empty".
+    false* lookup_empty.
+  - Case "G is not empty".
+    destruct (classicT (x = x0)) as [<- | Hn].
+    + SCase "x = x0".
+      pose proof (lookup_step_preservation_prec2 Hi Hwf (well_typed_push Hwt H H0 H1) Hs Ht eq_refl)
+        as [[S' [U' [u [[= ->] [Hv Hp']]]]] |
+            [[S' [ds [W [U' [G1 [G2 [pT [[=] [Hp' [Heq [Hds [Hrc1 Hrc2]]]]]]]]]]]] |
+             [q [r [r' [G1 [G2 [pT [[= <-] [-> [Heq [Hrc1 Hrc2]]]]]]]]]]]].
+      rewrite <- concat_empty_r in Heq at 1.
+      apply eq_sym in Heq. apply env_ok_inv in Heq as [<- [<- ->]]; try rewrite concat_empty_r in *; auto.
+      pose proof (sngl_typed2 Hi Hwf Ht) as [T [rx [rbs ->]]%precise_to_general2%typed_paths_named].
+      destruct Hrc1 as [-> | Hrc1];
+        destruct Hrc2 as [-> | [U Hu]%precise_to_general3%typing_implies_bound];
+        eauto.
+      * false binds_fresh_inv; eauto.
+      * apply sngl_typed3 in Hrc1 as
+            [? [S Hb]%precise_to_general3%typing_implies_bound].
+        false binds_fresh_inv; eauto. apply* inert_prefix. apply* wf_env_prefix.
+      * false binds_fresh_inv; eauto.
+    + SCase "x <> x0".
+      apply pt2_strengthen_one in Ht; auto.
+      apply lookup_strengthen_one in Hs; eauto. apply* IHHwt. apply* inert_prefix. apply* wf_env_prefix.
+Qed.
+
+Lemma wt_to_ok_s G s :
+  well_typed G s ->
+  ok s.
+Proof.
+  induction 1; eauto.
+Qed.
+
+Lemma typed_path_lookup_same_var2 G s y bs cs :
+  inert G ->
+  wf_env G ->
+  well_typed G s ->
+  G ⊢!! p_sel (avar_f y) bs : {{ p_sel (avar_f y) cs }} ->
+  s ⟦ p_sel (avar_f y) bs ⟼ defp (p_sel (avar_f y) cs) ⟧.
+Proof.
+  intros Hi Hwf Hwt Hp. pose proof (typ_to_lookup2 Hi Hwf Hwt Hp) as [t Hs].
+  pose proof (lookup_step_preservation_prec2 Hi Hwf Hwt Hs Hp eq_refl)
+        as [[? [? [? [[= ->] [Hv ->%pf_sngl_T]]]]] |
+            [[? [? [? [? [? [? [? [[= ->] [[=]%pf_sngl_T ?]]]]]]]]] |
+             [q' [r [r' [G1 [G2 [pT [-> [[= <-] [-> [Hrc1 Hrc2]]]]]]]]]]]]; auto.
+  - proof_recipe. inversions Hv. inversions H. inversion H0.
+  - apply (pt2_strengthen eq_refl Hi Hwf) in Hp.
+    pose proof (wt_prefix Hwt) as [v [s1 [s2 [-> Hwt']]]].
+    pose proof (wt_to_ok_s Hwt) as Hoks.
+    apply (lookup_strengthen Hoks eq_refl) in Hs.
+    pose proof (inert_ok Hi) as Hok%ok_middle_inv_l.
+    destruct Hrc1 as [<- | Hrc1]; destruct Hrc2 as [-> | Hrc2]; eauto.
+    + apply* lookup_step_weaken.
+    + apply (sngl_typed3 (inert_prefix (inert_prefix Hi))) in Hrc2
+        as [T [U Hb]%precise_to_general3%typing_implies_bound].
+      false binds_fresh_inv; eauto. repeat apply* wf_env_prefix.
+    + pose proof (typing_implies_bound (precise_to_general3 Hrc1)) as [S Hb].
+      false binds_fresh_inv; eauto.
+    + pose proof (typing_implies_bound (precise_to_general3 Hrc1)) as [S Hb].
+      false binds_fresh_inv; eauto.
+Qed.
+
+Lemma typed_path_lookup_same_var3 G s y bs cs :
+  inert G ->
+  wf_env G ->
+  well_typed G s ->
+  G ⊢!!! p_sel (avar_f y) bs : {{ p_sel (avar_f y) cs }} ->
+  s ⟦ defp (p_sel (avar_f y) bs) ⟼* defp (p_sel (avar_f y) cs) ⟧.
+Proof.
+  intros Hi Hwf Hwt Hp. dependent induction Hp.
+  - apply star_one. apply* typed_path_lookup_same_var2.
+  - pose proof (typed_paths_named (precise_to_general3 Hp)) as [qx [qbs ->]].
+    destruct (classicT (qx = y)) as [-> | Hn].
+    + pose proof (typed_path_lookup_same_var2 Hi Hwf Hwt H) as Hs.
+      specialize (IHHp _ _ _ Hi Hwf Hwt eq_refl eq_refl).
+      eapply star_trans. apply* star_one. auto.
+    + clear IHHp.
+      pose proof (typing_implies_bound (precise_to_general2 H)) as [S [G1 [G2 ->]]%binds_destruct].
+      pose proof (inert_ok Hi) as Hok%ok_middle_inv_l.
+      eapply pt2_strengthen in H; eauto.
+      pose proof (sngl_typed2 (inert_prefix Hi) (wf_env_prefix Hwf) H)
+        as [T [U [[-> ->] |
+                  [Hn' [G1' [G2' ->]]%binds_destruct]]%binds_push_inv]%precise_to_general2%typing_implies_bound].
+      * false*.
+      * do 2 rewrite <- concat_assoc in Hp, Hi, Hwf. apply (pt3_strengthen eq_refl Hi Hwf) in Hp.
+        apply (sngl_typed3 (inert_prefix Hi) (wf_env_prefix Hwf)) in Hp
+          as [V [W Hb]%precise_to_general3%typing_implies_bound].
+        simpl_dom. apply notin_union in Hok as [Hnu _]. false binds_fresh_inv; eauto.
+Qed.
+
+Lemma prev_var_exists G p q px pbs qx qbs:
+  inert G ->
+  wf_env G ->
+  p = p_sel (avar_f px) pbs ->
+  q = p_sel (avar_f qx) qbs ->
+  G ⊢!!! p : {{ q }} ->
+  px <> qx ->
+  exists p' cs q' ds rx,
+    rx <> px /\
+    p' = p_sel (avar_f px) cs /\
+    q' = p_sel (avar_f rx) ds /\
+    (p = p' \/ G ⊢!!! p : {{ p' }}) /\
+    G ⊢!! p' : {{ q' }} /\
+    (q' = q \/ G ⊢!!! q' : {{ q }}).
+Proof.
+  intros Hi Hwf -> -> Hp Hn. dependent induction Hp.
+  - repeat eexists; eauto.
+  - pose proof (sngl_typed2 Hi Hwf H) as [? [rx [rbs ->]]%precise_to_general2%typed_paths_named].
+    destruct (classicT (rx = qx)) as [-> | Hn'].
+    + do 5 eexists. split. eauto. split*.
+    + specialize (IHHp _ _ _ _ Hi Hwf eq_refl eq_refl Hn')
+        as [p' [cs [q' [ds [sx [Hn'' [-> [-> [Hp' [Hpq Hq]]]]]]]]]].
+      destruct (classicT (px = rx)) as [-> | Hnpr].
+      * eexists. exists cs. eexists. exists ds sx. repeat split*. right.
+        destruct Hp' as [<- | Hnr]; eauto.
+      * eexists. exists pbs. eexists. exists rbs rx. split*.
+Qed.
+
+Lemma typed_path_lookup_helper G s p r S T V :
+  inert G ->
+  wf_env G ->
+  well_typed G s ->
+  G ⊢!!! p : {{ r }} ->
+  G ⊢! r : ∀(S) T ⪼ V->
+  s ⟦ defp p ⟼* defp r ⟧.
+Proof.
+  intros Hi Hwf Hwt. gen p r S T V. induction Hwt; introv Hp Hr.
+  - Case "G is empty".
+    apply precise_to_general in Hr. false* typing_empty_false.
+  - Case "G is not empty".
+    destruct p as [x' bs].
+    pose proof (typed_paths_named (precise_to_general3 Hp)) as [px [pbs [= -> ->]]].
+    destruct (classicT (x = px)) as [-> | Hn].
+    + SCase "x = px".
+      lets Hwt': (well_typed_push Hwt H H0 H1).
+      pose proof (typ_to_lookup3 Hi Hwf Hwt' Hp) as [t Hlt].
+      pose proof (lookup_step_preservation_sngl_prec3 Hi Hwf Hwt' Hlt Hp Hr)
+        as [r1 [r2 [-> [Hrc Hrc']]]].
+      pose proof (sngl_typed3 Hi Hwf Hp) as [? [rx [rbs ->]]%precise_to_general3%typed_paths_named].
+      destruct (classicT (px = rx)) as [-> | Hn].
+      { apply* typed_path_lookup_same_var3. }
+      pose proof (prev_var_exists Hi Hwf eq_refl eq_refl Hp Hn) as
+          [p' [cs' [q' [ds [sx [Hn' [-> [-> [Hpp' [Hp'q' Hq'q]]]]]]]]]].
+      pose proof (typ_to_lookup2 Hi Hwf Hwt' Hp'q') as [t Hst].
+      pose proof (lookup_step_preservation_prec2 Hi Hwf Hwt' Hst Hp'q' eq_refl)
+        as [[S' [U' [u [[= ->] [Hv ->%pf_sngl_T]]]]] |
+            [[S' [ds' [W [U' [G1 [G2 [pT [-> [[=]%pf_sngl_T [Heq [Hds [Hrc1 Hrc2]]]]]]]]]]]] |
+             [q' [r [r' [G1 [G2 [pT [[= ->] [[= <-] [Heq' [Hrc1 Hrc2]]]]]]]]]]]]; auto.
+      { simpl in *. proof_recipe. inversions Hv. inversions H2. inversion H3. }
+      pose proof (inert_prefix Hi) as Hi'.
+      rewrite <- concat_empty_r in Heq' at 1. apply env_ok_inv'  in Heq' as [-> [-> <-]];
+                                               try rewrite concat_empty_r in *; auto.
+      assert (exists q'x q'bs, q' = p_sel (avar_f q'x) q'bs) as [q'x [q'bs ->]]. {
+        destruct Hrc2 as [-> | Hq'%precise_to_general3].
+        - destruct Hrc1 as [<- | Hq']; eauto.
+          pose proof (sngl_typed3 (inert_prefix Hi) (wf_env_prefix Hwf) Hq') as [? Hq''%precise_to_general3].
+          apply* typed_paths_named.
+        - apply* typed_paths_named.
+      }
+      assert (q'x <> px) as Hnqy. {
+        intros ->. pose proof (lookup_same_var_same_type Hi Hwf Hwt' Hst Hp'q') as [= -> ->]. false*.
+      }
+      apply star_trans with (b:=defp (p_sel (avar_f px) cs')). {
+        destruct Hpp' as [[= ->] | Hpp'].
+        - apply* star_refl.
+        - eapply (typed_path_lookup_same_var3 Hi); auto.
+      }
+      clear Hpp'.
+      assert (p_sel (avar_f rx) rbs = r2) as <-. {
+        destruct Hrc as [<- | Ht]; auto. false (pf_inert_pt3_sngl_false Hi Hr Ht); auto.
+      }
+      clear Hrc.
+      apply star_trans with (b:=defp (p_sel (avar_f q'x) q'bs)).
+      { apply* star_one. }
+      apply* lookup_weaken.
+      { apply* wt_to_ok_s. }
+      pose proof (wf_env_prefix Hwf) as Hwf'.
+      apply pf_strengthen in Hr; auto. clear Hrc' Hst Hp'q' Hp.
+      destruct Hq'q as [[= -> ->] | Hq'q%pt3_strengthen_one]; destruct Hrc1 as [<- | Hrc1]; destruct Hrc2 as [[= ->] | Hrc2]; subst; auto;
+        [ apply* star_refl | ..];
+        try solve [apply* IHHwt; try solve [false (pf_inert_pt3_sngl_false Hi' Hr Hrc1); auto]].
+        * apply* IHHwt. apply* pt3_sngl_trans3.
+        * pose proof (pt3_invert Hi' Hrc1 Hq'q) as [Contra | [q' [[= ->] [[= <-] | Hqt]]]].
+          ** false (pf_inert_pt3_sngl_false Hi' Hr Contra); auto.
+          ** subst. apply* star_refl.
+          ** apply* IHHwt.
+        * pose proof (pt3_invert Hi' Hrc1 Hq'q) as [Contra | [q' [[= ->] [[= <-] | Hqt]]]].
+          ** false (pf_inert_pt3_sngl_false Hi' Hr Contra); auto.
+          ** apply* IHHwt.
+          ** apply (pt3_sngl_trans3 Hrc2) in Hqt. apply* IHHwt.
+    + SCase "x <> px".
+      apply pt3_strengthen_one in Hp; auto. apply lookup_weaken.
+      { apply* ok_push. apply* wt_to_ok_s. }
+      pose proof (inert_prefix Hi) as Hi'. pose proof (wf_env_prefix Hwf) as Hwf'.
+      apply* IHHwt.
+      apply (sngl_typed3 Hi' Hwf') in Hp as [U Ht]. apply* pf_strengthen_from_pt3.
+Qed.
+
+Lemma last_path G p T U :
+  inert G ->
+  G ⊢!!! p : ∀(T) U ->
+  G ⊢!! p : ∀(T) U \/ exists q, G ⊢!!! p: {{ q }} /\ G ⊢!! q : ∀(T) U.
+Proof.
+  intros Hi Hp. dependent induction Hp; eauto.
+  specialize (IHHp _ _ Hi eq_refl) as [Hq | [r [Hq Hr]]]; eauto.
+Qed.
+
+Lemma typed_path_lookup3 G s p T U :
+  inert G ->
+  wf_env G ->
+  well_typed G s ->
+  G ⊢!!! p: ∀(T) U ->
+  exists v, s ∋ (p, v).
+Proof.
+  intros Hi Hwf Hwt Hp.
+  pose proof (typed_paths_named (precise_to_general3 Hp)) as [px [pbs ->]].
+  apply (last_path Hi) in Hp as [Hp | [q [Hpq Hq]]].
+  - inversions Hp. pose proof (typ_to_lookup1 Hi Hwf Hwt H) as [t Hs].
+    destruct (lookup_step_preservation_prec1 Hi Hwf Hwt Hs H eq_refl)
+          as [[S [u [-> Ht]]] |
+              [[S [ds' [W [T'' [G1 [G2 [pT [-> [[= ->] [? ?]]]]]]]]]] |
+               [? [? [? [? [? [? [? [[= ->] [-> ?]]]]]]]]]]].
+    + eexists. constructor. apply* star_one.
+    + eexists. constructor. apply* star_one.
+    + apply pf_sngl_U in H as [=].
+  - inversions Hq. pose proof (pf_forall_T Hi H) as ->.
+    pose proof (typed_path_lookup_helper Hi Hwf Hwt Hpq H) as Hs.
+    pose proof (typ_to_lookup1 Hi Hwf Hwt H) as [t Hs'].
+    pose proof (typed_paths_named (precise_to_general H)) as [qx [qbs ->]].
+    destruct (lookup_step_preservation_prec1 Hi Hwf Hwt Hs' H eq_refl)
+          as [[S [u [-> Ht]]] |
+              [[S [ds' [W [T'' [G1 [G2 [pT [-> [[= ->] [? ?]]]]]]]]]] |
+               [? [? [? [? [? [? [? [[= ->] [-> ?]]]]]]]]]]].
+    eexists. constructor. eapply star_trans. apply Hs. apply* star_one.
+Qed.
+
+
+(** * Lemmas to Prove Canonical Forms for Functions *)
+
+Lemma lookup_preservation_forall : forall G s t u T S,
+    inert G ->
+    wf_env G ->
+    well_typed G s ->
+    star (lookup_step s) t u ->
+    G ⊢ deftrm t : ∀(S) T ->
+    G ⊢ deftrm u: ∀(S) T.
+Proof.
+  introv Hi Hwf Hwt Hl Hp. dependent induction Hl; auto.
+  assert (exists q, a = defp q) as [q ->] by (inversions H; eauto).
+  proof_recipe.
+  apply repl_to_precise_typ_all in Hp as [S' [T' [? [Hpr' [? ?]]]]]; auto.
+  apply IHHl.
+  pose proof (lookup_step_preservation_prec3_fun Hi Hwf Hwt H Hpr') as Hb.
+  apply ty_sub with (T:=∀(S') T'); auto; fresh_constructor; apply* tight_to_general.
+Qed.
+
+Lemma corresponding_types_fun: forall G s p S T,
+    inert G ->
+    wf_env G ->
+    well_typed G s ->
+    G ⊢!!! p: ∀(S) T ->
+    (exists v, s ∋ (p, v) /\
+            G ⊢ trm_val v : ∀(S) T).
+Proof.
+  introv Hi Hwf Hwt Hp.
+  destruct (typed_path_lookup3 Hi Hwf Hwt Hp) as [v Hs].
+  inversions Hs.
+  lets Ht: (lookup_preservation_forall Hi Hwf Hwt H1 (precise_to_general3 Hp)). eauto.
+Qed.
+
+(** [forall] to [G(x)]        #<br>#
+    [inert G]            #<br>#
+    [G ⊢ p: forall(T)U]       #<br>#
+    [――――――――――――――--]   #<br>#
+    [exists T', U',]          #<br>#
+    [G ∋ (p, forall(T')U')]   #<br>#
+    [G ⊢ T <: T']        #<br>#
+    [forall fresh y, G, y: T ⊢ U'^y <: U^y] *)
+Lemma path_typ_all_to_binds: forall G p T U,
+    inert G ->
+    G ⊢ trm_path p : ∀(T) U ->
+    (exists L T' U',
+        G ⊢!!! p : ∀(T') U' /\
+        G ⊢ T <: T' /\
+        (forall y, y \notin L -> G & y ~ T ⊢ (open_typ y U') <: (open_typ y U))).
+Proof.
+  introv Hin Ht.
+  lets Htt: (general_to_tight_typing Hin Ht).
+  lets Hrepl: (replacement_closure Hin Htt).
+  destruct (repl_to_precise_typ_all Hin Hrepl) as [T' [U' [L [Hs1 [Hs2 Hs3]]]]].
+  exists L T' U'. repeat split; auto.
+  apply* tight_to_general.
+Qed.
+
+(** [forall] to [lambda]                 #<br>#
+    [inert G]                       #<br>#
+    [G ⊢ v: forall(T)U]                  #<br>#
+    [――――――――――――]                  #<br>#
+    [exists T', t,]                      #<br>#
+    [v = lambda(T')t]               #<br>#
+    [G ⊢ T <: T']                   #<br>#
+    [forall fresh y, G, y: T ⊢ t^y: U^y] *)
+Lemma val_typ_all_to_lambda: forall G v T U,
+    inert G ->
+    G ⊢ trm_val v : ∀(T) U ->
+    (exists L T' t,
+        v = λ(T') t /\
+        G ⊢ T <: T' /\
+        (forall y, y \notin L -> G & y ~ T ⊢ (open_trm y t) : open_typ y U)).
+Proof.
+  introv Hin Ht. proof_recipe. inversions Hvpr.
+  exists (L1 \u L \u (dom G)) S1 t. repeat split~.
+  intros. assert (HL: y \notin L) by auto. assert (HL0: y \notin L1) by auto.
+  specialize (HS2 y HL0).
+  specialize (H2 y HL).
+  eapply ty_sub; eauto. eapply narrow_typing in H2; eauto.
+Qed.
