src/extensions/paths-no-closure-os/Examples.v
@@ -1,0 +1,205 @@
+Require Import Definitions Binding Weakening.
+Require Import List.
+
+Section ListExample.
+
+Variables A List : typ_label.
+Variables Nil Cons head tail : trm_label.
+
+Hypothesis NC: Nil <> Cons.
+Hypothesis HT: head <> tail.
+
+
+Notation this := (p_sel (avar_b 0) nil).
+Notation super := (p_sel (avar_b 1) nil).
+Notation ssuper := (p_sel (avar_b 2) nil).
+Notation sssuper := (p_sel (avar_b 3) nil).
+Notation ssssuper := (p_sel (avar_b 4) nil).
+Notation sssssuper := (p_sel (avar_b 5) nil).
+
+Notation lazy t := (defv (λ(⊤) t)).
+Notation Lazy T := (∀(⊤) T).
+
+Notation ListTypeA list_level A_lower A_upper A_level :=
+  (typ_rcd { A >: A_lower <: A_upper } ∧
+   typ_rcd { head ⦂ Lazy (super↓A) } ∧
+   typ_rcd { tail ⦂ Lazy (list_level↓List ∧ typ_rcd { A >: ⊥ <: A_level↓A }) }).
+Notation ListType list_level := (ListTypeA list_level ⊥ ⊤ super).
+
+Notation "d1 'Λ' d2" := (defs_cons d1 d2) (at level 40).
+
+Notation ListObjType :=
+  (typ_rcd { List >: μ (ListType ssuper) <: μ (ListType ssuper) } ∧
+   typ_rcd { Nil  ⦂ ∀(typ_rcd { A >: ⊥ <: ⊤ }) (super↓List ∧ (typ_rcd { A >: ⊥ <: this↓A })) } ∧
+   typ_rcd { Cons ⦂ ∀(typ_rcd { A >: ⊥ <: ⊤ })                       (* x: {A} *)
+                    ∀(this↓A)                                        (* y: x.A *)
+                    ∀(ssuper↓List ∧ typ_rcd { A >: ⊥ <: super↓A })   (* ys: sci.List ∧ {A <: x.A} *)
+                     (sssuper↓List ∧ typ_rcd { A >: ⊥ <: ssuper↓A }) }).
+
+Definition t :=
+ trm_val (ν (ListObjType)
+            defs_nil Λ
+            { List ⦂= μ (ListType ssuper) } Λ
+            { Nil := defv (λ(typ_rcd { A >: ⊥ <: ⊤ })
+                            trm_let (* result = *)
+                            (trm_val (ν(ListTypeA sssuper (super↓A) (super↓A) super)
+                                       defs_nil Λ
+                                       { A ⦂= super↓A } Λ
+                                       { head := defv (λ(⊤) trm_app super•head this) } Λ
+                                       { tail := defv (λ(⊤) trm_app super•tail this) }))
+                            (trm_path this)) } Λ
+            { Cons := defv (λ(typ_rcd { A >: ⊥ <: ⊤ })
+                   trm_val (λ(this↓A)
+                   trm_val (λ(ssuper↓List ∧ typ_rcd { A >: ⊥ <: super↓A })
+                             trm_let (* result = *)
+                             (trm_val (ν(ListTypeA sssssuper (sssuper↓A) (sssuper↓A) ssssuper)
+                                        defs_nil Λ
+                                        { A ⦂= sssuper↓A } Λ
+                                        { head := lazy (trm_path sssuper) } Λ
+                                        { tail := lazy (trm_path ssuper)}))
+                             (trm_path this)))) }).
+
+
+Lemma list_typing :
+  empty ⊢ t : μ ListObjType.
+Proof.
+  fresh_constructor. repeat apply ty_defs_cons; auto.
+  - Case "Nil".
+    constructor. fresh_constructor. simpl. repeat case_if.
+    unfold open_trm, open_typ. simpl. repeat case_if.
+    (* ⊢ let result = ν(ListType){A}{head}{tail} in result : List ∧ {A <:} *)
+    fresh_constructor.
+    + (* ⊢ ν(ListType){A}{head}{tail} in result : μ(ListType) *)
+      fresh_constructor. repeat apply ty_defs_cons; simpl; auto.
+      * SCase "head".
+        constructor. fresh_constructor. case_if. unfold open_trm, open_typ. simpl. repeat case_if. simpl. case_if.
+        assert (p_sel (avar_f y0) nil ↓ A = open_typ_p (p_sel (avar_f y1) nil) (p_sel (avar_f y0) nil ↓ A))
+          as Heq by (unfold open_typ_p; auto).
+        rewrite Heq. eapply ty_all_elim.
+        ** rewrite proj_rewrite. apply ty_new_elim.
+           eapply ty_sub; try solve [constructor*].
+           eapply subtyp_trans.
+           { apply subtyp_and11. }
+           apply subtyp_and12.
+        ** eapply ty_sub.
+           { constructor*. }
+           auto.
+      * unfold defs_hasnt. simpl. case_if*.
+      * SCase "tail".
+        repeat case_if. constructor. fresh_constructor.
+        unfold open_trm, open_typ. simpl. repeat case_if.
+        assert ((p_sel (avar_f z) nil ↓ List) ∧ typ_rcd {A >: ⊥ <: p_sel (avar_f y0) nil ↓ A} =
+                open_typ_p (p_sel (avar_f y1) nil)
+                           ((p_sel (avar_f z) nil ↓ List) ∧ typ_rcd {A >: ⊥ <: p_sel (avar_f y0) nil ↓ A}))
+          as Heq by (unfold open_typ_p; auto).
+        rewrite Heq. eapply ty_all_elim.
+        ** rewrite proj_rewrite. apply ty_new_elim.
+           eapply ty_sub; try solve [constructor*].
+        ** eapply ty_sub.
+           { constructor*. }
+           auto.
+      * unfold defs_hasnt. simpl. repeat case_if; auto.
+    + (* y0: ListType ⊢ y0: List ∧ {A<:} *)
+      match goal with
+      | H: _ |- ?G' ⊢ _ : _ =>
+        remember G' as G
+      end.
+      unfold open_trm. simpl. case_if.
+      remember (p_sel (avar_f y0) nil) as py0.
+      assert (G ⊢ trm_path py0 : typ_rcd {A >: p_sel (avar_f y) nil ↓ A <: p_sel (avar_f y) nil ↓ A}) as Hpy1. {
+        rewrite Heqpy0, HeqG.
+        eapply ty_sub. apply ty_rec_elim. constructor*.
+        unfold open_typ_p. simpl. case_if. eapply subtyp_trans; apply subtyp_and11.
+      }
+      assert (G ⊢ trm_path py0 : typ_rcd { head ⦂ Lazy (p_sel (avar_f y0) nil ↓ A) }) as Hpy2. {
+        rewrite Heqpy0, HeqG.
+        eapply ty_sub. apply ty_rec_elim. constructor*.
+        unfold open_typ_p. simpl. case_if. eapply subtyp_trans. apply subtyp_and11. eauto.
+      }
+      assert (G ⊢ trm_path py0 : typ_rcd {tail ⦂ Lazy ((p_sel (avar_f z) nil ↓ List) ∧
+                                                       typ_rcd {A >: ⊥ <: p_sel (avar_f y0) nil ↓ A})}) as Hpy3. {
+        rewrite Heqpy0, HeqG.
+        eapply ty_sub. apply ty_rec_elim. constructor*.
+        unfold open_typ_p. simpl. case_if. apply subtyp_and12.
+      }
+      apply ty_and_intro.
+      * apply ty_sub with (T:=μ ListType (p_sel (avar_f z) nil)).
+        ** apply ty_rec_intro. unfold open_typ_p. simpl. case_if.
+           apply ty_and_intro.
+           { apply ty_and_intro.
+             - apply (ty_sub Hpy1). eauto.
+             - rewrite Heqpy0 in *. auto.
+           }
+           rewrite Heqpy0 in *. auto.
+        ** eapply subtyp_sel2.
+           eapply ty_sub.
+           {
+             rewrite HeqG.
+             constructor*.
+           }
+           eapply subtyp_trans; apply subtyp_and11.
+      * eapply ty_sub. apply Hpy1. apply subtyp_typ; auto.
+  - unfold defs_hasnt. simpl. case_if. auto.
+  - Case "Cons".
+    constructor. do 4 (fresh_constructor; unfold open_trm, open_typ; simpl; repeat case_if).
+    (* ⊢ let result = ν(ListType){A}{head}{tail} in result : List ∧ {A <:} *)
+    + (* ⊢ ν(ListType){A}{head}{tail} in result : μ(ListType) *)
+      fresh_constructor. repeat apply ty_defs_cons; simpl; auto.
+      * SCase "head".
+        case_if.
+        constructor. fresh_constructor. unfold open_trm, open_typ. simpl.
+        case_if.
+        eapply ty_sub.
+        { constructor*. }
+        eapply subtyp_sel2. eapply ty_sub.
+        constructor*. eapply subtyp_trans. apply subtyp_and11. eauto.
+      * unfold defs_hasnt. simpl. case_if. auto.
+      * SCase "tail".
+        constructor. fresh_constructor. unfold open_trm, open_typ. simpl. case_if.
+        apply ty_and_intro.
+        ** eapply ty_sub. constructor*. eauto.
+        ** eapply ty_sub. eapply ty_sub. constructor*. apply subtyp_and12. apply subtyp_typ.
+           auto. auto.
+      * unfold defs_hasnt. simpl. repeat case_if. auto.
+    + (* y2: ListType ⊢ y2: List ∧ {A<:} *)
+       match goal with
+      | H: _ |- ?G' ⊢ _ : _ =>
+        remember G' as G
+      end.
+      unfold open_trm. simpl. case_if.
+      remember (p_sel (avar_f y2) nil) as py0.
+      assert (G ⊢ trm_path py0 : typ_rcd {A >: p_sel (avar_f y) nil ↓ A <: p_sel (avar_f y) nil ↓ A}) as Hpy1. {
+        rewrite Heqpy0, HeqG.
+        eapply ty_sub. apply ty_rec_elim. constructor*.
+        unfold open_typ_p. simpl. case_if. eapply subtyp_trans; apply subtyp_and11.
+      }
+      assert (G ⊢ trm_path py0 : typ_rcd { head ⦂ Lazy (p_sel (avar_f y2) nil ↓ A) }) as Hpy2. {
+        rewrite Heqpy0, HeqG.
+        eapply ty_sub. apply ty_rec_elim. constructor*.
+        unfold open_typ_p. simpl. case_if. eapply subtyp_trans. apply subtyp_and11. eauto.
+      }
+      assert (G ⊢ trm_path py0 : typ_rcd {tail ⦂ Lazy ((p_sel (avar_f z) nil ↓ List) ∧
+                                                       typ_rcd {A >: ⊥ <: p_sel (avar_f y) nil ↓ A})}) as Hpy3. {
+        rewrite Heqpy0, HeqG.
+        eapply ty_sub. apply ty_rec_elim. constructor*.
+        unfold open_typ_p. simpl. case_if. apply subtyp_and12.
+      }
+      apply ty_and_intro.
+      * apply ty_sub with (T:=μ ListType (p_sel (avar_f z) nil)).
+        ** rewrite Heqpy0 in *. apply ty_rec_intro. unfold open_typ_p. simpl. case_if.
+           apply ty_and_intro.
+           { apply ty_and_intro; auto. apply (ty_sub Hpy1). eauto. }
+           eapply ty_sub. apply Hpy3.
+           constructor. fresh_constructor.
+           unfold open_typ. simpl. apply subtyp_and2.
+           *** apply subtyp_and11.
+           *** eapply subtyp_trans. apply subtyp_and12. apply subtyp_typ. auto.
+               eapply subtyp_sel2. apply* weaken_ty_trm. rewrite HeqG. repeat apply* ok_push.
+        ** rewrite HeqG in *.
+           eapply subtyp_sel2. eapply ty_sub. constructor*.
+           eapply subtyp_trans. apply subtyp_and11. eapply subtyp_and11.
+      * eapply ty_sub. apply Hpy1. apply subtyp_typ; auto.
+  - simpl. repeat case_if. unfold defs_hasnt. simpl. repeat case_if. auto.
+Qed.
+
+End ListExample.
