src/extensions/paths-no-closure-os/GeneralToTight.v
@@ -1,0 +1,209 @@
+(** printing |-#    %\vdash_{\#}%    #&vdash;<sub>&#35;</sub>#     *)
+(** printing |-##   %\vdash_{\#\#}%  #&vdash;<sub>&#35&#35</sub>#  *)
+(** printing |-##v  %\vdash_{\#\#v}% #&vdash;<sub>&#35&#35v</sub># *)
+(** printing |-!    %\vdash_!%       #&vdash;<sub>!</sub>#         *)
+(** remove printing ~ *)
+
+Set Implicit Arguments.
+
+Require Import Sequences.
+Require Import Coq.Program.Equality.
+Require Import Definitions RecordAndInertTypes PreciseTyping TightTyping InvertibleTyping
+        Replacement ReplacementTyping.
+
+Lemma pt2_dec_typ_tight: forall G p A S U,
+    inert G ->
+    G ⊢!! p: typ_rcd {A >: S <: U} ->
+    S = U.
+Proof.
+  introv Hi Hp. dependent induction Hp; eauto. apply* pf_dec_typ_tight.
+Qed.
+
+Lemma pt3_dec_typ_tight: forall G p A S U,
+    inert G ->
+    G ⊢!!! p: typ_rcd {A >: S <: U} ->
+    S = U.
+Proof.
+  introv Hi Hp. dependent induction Hp; eauto. apply* pt2_dec_typ_tight.
+Qed.
+
+(** * Sel-<: Premise
+    This lemma corresponds to Lemma 3.5 in the paper.
+
+    [inert G]                    #<br>#
+    [G |-## x: {A: S..U}]        #<br>#
+    [――――――――――――――――――――――――――――]   #<br>#
+    [exists T. G |-## x: {A: T..T}]   #<br>#
+    [G |-# T <: U]               #<br>#
+    [G |-# S <: T]                    *)
+Lemma sel_premise_inv: forall G p A S U,
+  inert G ->
+  G ⊢## p : typ_rcd {A >: S <: U} ->
+  exists T,
+    G ⊢!!! p : typ_rcd {A >: T <: T} /\
+    G ⊢# T <: U /\
+    G ⊢# S <: T.
+Proof.
+  introv HG Hinv.
+  dependent induction Hinv.
+  - lets Hp: (pt3_dec_typ_tight HG H). subst.
+    exists U. split*.
+  - specialize (IHHinv _ _ _ HG eq_refl).
+    destruct IHHinv as [V [Hx [Hs1 Hs2]]].
+    exists V. split*.
+Qed.
+
+Lemma sel_premise: forall G p A S U,
+  inert G ->
+  G ⊢// p : typ_rcd {A >: S <: U} ->
+  exists T,
+    G ⊢!!! p : typ_rcd {A >: T <: T} /\
+    G ⊢# T <: U /\
+    G ⊢# S <: T.
+Proof.
+  introv HG Hr. dependent induction Hr.
+  apply* sel_premise_inv.
+Qed.
+
+(** * Sel-<: Replacement
+    This lemma corresponds to Lemma 3.4 in the paper.
+
+    [inert G]              #<br>#
+    [G ⊢# x: {A: S..U}]   #<br>#
+    [――――――――――――――――――――――]   #<br>#
+    [G ⊢# x.A <: U]       #<br>#
+    [G ⊢# S <: x.A]            *)
+Lemma sel_replacement: forall G p A S U,
+    inert G ->
+    G ⊢# trm_path p : typ_rcd {A >: S <: U} ->
+    (G ⊢# p↓A <: U /\
+     G ⊢# S <: p↓A).
+Proof.
+  introv Hi Hty.
+  pose proof (replacement_closure Hi Hty) as Hinv.
+  pose proof (sel_premise Hi Hinv) as [T [Ht [Hs1 Hs2]]].
+  split.
+  - apply subtyp_sel1_t in Ht. apply subtyp_trans_t with (T:=T); auto.
+  - apply subtyp_sel2_t in Ht. apply subtyp_trans_t with (T:=T); auto.
+Qed.
+
+Lemma tight_to_prec_exists G p T :
+  inert G ->
+  G ⊢# trm_path p : T ->
+  exists U, G ⊢!! p : U.
+Proof.
+  intros Hi Hp. pose proof (replacement_closure Hi Hp).
+  apply repl_to_inv in H as [? ?]. apply inv_to_prec in H as [? ?]. apply* pt2_exists.
+Qed.
+
+Lemma sngl_replacement: forall G p q n T U S,
+    inert G ->
+    G ⊢# trm_path p: {{ q }} ->
+    G ⊢# trm_path q : S ->
+    repl_typ n p q T U ->
+    G ⊢# T <: U /\ G ⊢# U <: T.
+Proof.
+  introv Hi Hp Hr.
+  apply (tight_to_prec_exists Hi) in Hr as [V Hq].
+  lets Hc: (replacement_closure Hi Hp).
+  pose proof (repl_to_invertible_sngl Hi Hc Hq) as [r [W [Hpt [Hq' [-> | Hpq]]]]];
+    pose proof (inv_to_precise_sngl Hi Hpt (pt3 Hq')) as [r' [Ht [-> | Hrc']]].
+  - split. eauto. apply repl_swap in H. eauto.
+  - split.
+    + destruct (repl_insert r H) as [X [Hr1 Hr2]].
+      eapply subtyp_sngl_pq_t. eapply pt3_sngl_trans3. apply Ht. eauto. eauto. eauto.
+    + destruct (repl_insert r' H) as [X [Hr1 Hr2]].
+      apply subtyp_trans_t with (T:=X).
+      * apply repl_swap in Hr2. eauto.
+      * apply repl_swap in Hr1. eauto.
+  - split.
+    + destruct (repl_insert r H) as [X [Hr1 Hr2]].
+      apply subtyp_trans_t with (T:=X); eauto.
+    + destruct (repl_insert r H) as [X [Hr1 Hr2]].
+      apply subtyp_trans_t with (T:=X).
+      apply repl_swap in Hr2. eauto. apply repl_swap in Hr1. eauto.
+  - split.
+    + destruct (repl_insert r' H) as [X [Hr1 Hr2]].
+      apply subtyp_trans_t with (T:=X).
+      * eauto.
+      * destruct (repl_insert r Hr2) as [S' [Hr1' Hr2']].
+        apply subtyp_trans_t with (T:=S'); eauto.
+    + destruct (repl_insert r H) as [X [Hr1 Hr2]].
+      apply subtyp_trans_t with (T:=X).
+      * apply repl_swap in Hr2. eauto.
+      * destruct (repl_insert r' Hr1) as [S' [Hr1' Hr2']].
+        apply subtyp_trans_t with (T:=S').
+        ** apply repl_swap in Hr2'. eauto.
+        ** apply repl_swap in Hr1'. eauto.
+Qed.
+
+(** * General to Tight [⊢ to ⊢#] *)
+(** The following lemma corresponds to Theorem 3.3 in the paper.
+    It says that in an inert environment, general typing ([ty_trm] [⊢]) can
+    be reduced to tight typing ([ty_trm_t] [⊢#]).
+    The proof is by mutual induction on the typing and subtyping judgements.
+
+    [inert G]           #<br>#
+    [G ⊢ t: T]          #<br>#
+    [――――――――――――――]    #<br>#
+    [G ⊢# t: T] #<br># #<br>#
+
+    and                 #<br># #<br>#
+    [inert G]           #<br>#
+    [G ⊢ S <: U]        #<br>#
+    [――――――――――――――――]  #<br>#
+    [G ⊢# S <: U]         *)
+Lemma general_to_tight: forall G0,
+  inert G0 ->
+  (forall G t T,
+     G ⊢ t : T ->
+     G = G0 ->
+     G ⊢# t : T) /\
+  (forall G S U,
+     G ⊢ S <: U ->
+     G = G0 ->
+     G ⊢# S <: U).
+Proof.
+  intros G0 Hi.
+  apply ts_mutind; intros; subst;
+    try solve [eapply sel_replacement; auto]; eauto.
+  - destruct* (sngl_replacement Hi (H eq_refl) (H0 eq_refl) r).
+  - apply repl_swap in r. destruct* (sngl_replacement Hi (H eq_refl) (H0 eq_refl) r).
+Qed.
+
+(** The general-to-tight lemma, formulated for term typing. *)
+Lemma general_to_tight_typing: forall G t T,
+  inert G ->
+  G ⊢ t : T ->
+  G ⊢# t : T.
+Proof.
+  intros. apply* general_to_tight.
+Qed.
+
+Ltac proof_recipe :=
+  match goal with
+  | [ Hg: ?G ⊢ _ : _,
+      Hi: inert ?G |- _ ] =>
+    apply (general_to_tight_typing Hi) in Hg;
+    ((apply (replacement_closure Hi) in Hg) || (apply (replacement_closure_v Hi) in Hg));
+    try lets Hok: (inert_ok Hi);
+    try match goal with
+        | [ Hr: ?G ⊢// _ : ∀(_) _,
+            Hok: ok ?G |- _ ] =>
+          destruct (repl_to_precise_typ_all Hi Hr) as [Spr [Tpr [Lpr [Hpr [Hspr1 Hspr2]]]]]
+        | [ Hrv: ?G ⊢//v _ : μ _ |- _ ] =>
+          apply (repl_to_invertible_obj Hi) in Hrv as [U' [Hrv Hrc]];
+          apply (invertible_to_precise_obj Hi) in Hrv as [U'' [Hrv Hrc']];
+          try match goal with
+              | [ Hv: _ ⊢!v val_new ?T _ : μ ?U |- _ ] =>
+                assert (T = U) as <- by (inversion Hv; subst*)
+              end
+        | [ Hrv: ?G ⊢//v _ : ∀(_) _ |- _ ] =>
+          inversions Hrv;
+          match goal with
+          | [ Hrv: ?G ⊢##v _ : ∀(_) _,
+              Hok: ok ?G |- _ ] =>
+            apply invertible_val_to_precise_lambda in Hrv as [L1 [S1 [T1 [Hvpr [HS1 HS2]]]]]; auto
+          end
+       end
+  end.
