src/extensions/paths-no-closure-os/LocalClosure.v
@@ -1,0 +1,75 @@
+(** printing |-#    %\vdash_{\#}%    #&vdash;<sub>&#35;</sub>#     *)
+(** printing |-##   %\vdash_{\#\#}%  #&vdash;<sub>&#35&#35</sub>#  *)
+(** printing |-##v  %\vdash_{\#\#v}% #&vdash;<sub>&#35&#35v</sub># *)
+(** printing |-!    %\vdash_!%       #&vdash;<sub>!</sub>#         *)
+(** remove printing ~ *)
+Set Implicit Arguments.
+
+Require Import Definitions.
+
+(** * Local Closure
+  Our definition of [trm] accepts terms that contain de Bruijn indices that are unbound.
+  A symbol [X] is considered locally closed, denoted [lc X], if all de Bruijn indices
+  in [X] are bound.
+   We will require a term to be locally closed in the final safety theorem. *)
+
+(** Only named variables are locally closed. *)
+Inductive lc_var : avar -> Prop :=
+| lc_var_x : forall x,
+    lc_var (avar_f x).
+
+Inductive lc_path : path -> Prop :=
+| lc_p: forall x bs,
+    lc_var x ->
+    lc_path (p_sel x bs).
+
+(** Locally closed types and declarations. *)
+Inductive lc_typ : typ -> Prop :=
+| lc_typ_top : lc_typ ⊤
+| lc_typ_bot : lc_typ ⊥
+| lc_typ_rcd : forall D,
+    lc_dec D ->
+    lc_typ (typ_rcd D)
+| lc_typ_and : forall T1 T2,
+    lc_typ T1 ->
+    lc_typ T2 ->
+    lc_typ (T1 ∧ T2)
+| lc_typ_path : forall p L,
+    lc_path p ->
+    lc_typ (p↓L)
+| lc_typ_bnd : forall T,
+    (forall x, lc_typ (open_typ x T)) ->
+    lc_typ (μ T)
+| lc_typ_all : forall T1 T2,
+    (forall x, lc_typ (open_typ x T2)) ->
+    lc_typ T1 ->
+    lc_typ (∀(T1) T2)
+with lc_dec : dec -> Prop :=
+| lc_dec_typ : forall A T U,
+    lc_typ T ->
+    lc_typ U ->
+    lc_dec { A >: T <: U }
+| lc_dec_trm : forall a T,
+    lc_typ T ->
+    lc_dec {a ⦂ T}.
+
+Inductive lc_ctx : ctx -> Prop :=
+| lc_ctx_empty : lc_ctx empty
+| lc_ctx_push : forall G x T,
+  lc_ctx G -> lc_typ T -> lc_ctx (G & x ~ T).
+
+Definition lc_ctx' G := forall x T, binds x T G -> lc_typ T.
+
+Hint Constructors lc_var lc_path lc_typ lc_dec lc_ctx.
+
+(*
+Scheme lc_trm_mut  := Induction for lc_trm Sort Prop
+with   lc_val_mut  := Induction for lc_val Sort Prop
+with   lc_def_mut  := Induction for lc_def Sort Prop
+with   lc_defs_mut := Induction for lc_defs Sort Prop.
+Combined Scheme lc_mutind from lc_trm_mut, lc_val_mut, lc_def_mut, lc_defs_mut.
+
+Scheme lc_typ_mut := Induction for lc_typ Sort Prop
+with   lc_dec_mut := Induction for lc_dec Sort Prop.
+Combined Scheme lc_typ_mutind from lc_typ_mut, lc_dec_mut.
+*)
